theories/lang.v
@@ -12,59 +12,79 @@ Inductive mode := i |o.
 Inductive S :=  b of B | arr of mode & S & S.
 Notation "x '--i-->' y" := (arr i x y) (at level 3).
 Notation "x '--o-->' y" := (arr o x y) (at level 3).
+derive D.
+Elpi derive.eqbOK.register_axiom D is_D is_nat_inhab D_eqb D_eqb_correct D_eqb_refl.
+HB.instance Definition _ := hasDecEq.Build D D_eqb_OK.
+derive mode.
+Elpi derive.eqbOK.register_axiom mode is_mode is_nat_inhab mode_eqb mode_eqb_correct mode_eqb_refl.
+HB.instance Definition _ := hasDecEq.Build mode mode_eqb_OK.
+(* derive S.
+Elpi derive.eqbOK.register_axiom S is_S is_nat_inhab S_eqb S_eqb_correct S_eqb_refl.
+HB.instance Definition _ := hasDecEq.Build S S_eqb_OK. *)
 
-Definition P := nat.
-derive P.
-Elpi derive.eqbOK.register_axiom P is_P is_nat_inhab P_eqb P_eqb_correct P_eqb_refl.
+Inductive Kp := IKp : nat -> Kp.
+derive Kp.
+Elpi derive.eqbOK.register_axiom Kp is_Kp is_nat_inhab Kp_eqb Kp_eqb_correct Kp_eqb_refl.
+HB.instance Definition _ := hasDecEq.Build Kp Kp_eqb_OK.
 
-Definition K := nat.
-derive K.
-Elpi derive.eqbOK.register_axiom K is_K is_nat_inhab K_eqb K_eqb_correct K_eqb_refl.
+Inductive Kd := IKd : nat -> Kd.
+derive Kd.
+Elpi derive.eqbOK.register_axiom Kd is_Kd is_nat_inhab Kd_eqb Kd_eqb_correct Kd_eqb_refl.
+HB.instance Definition _ := hasDecEq.Build Kd Kd_eqb_OK.
 
-Definition V := nat.
+Inductive V := IV : nat -> V.
 derive V.
 Elpi derive.eqbOK.register_axiom V is_V is_nat_inhab V_eqb V_eqb_correct V_eqb_refl.
+HB.instance Definition _ := hasDecEq.Build V V_eqb_OK.
 
-Inductive C := 
-  | p of P 
-  | v of V
-  .
-derive C.
 
 Inductive Tm := 
-  | Code : C -> Tm
-  | Data : K -> Tm
-  | Comb : Tm -> Tm -> Tm.
-  (* | Lam  : V -> S -> Tm -> S -> Tm. *)
+  | Tm_Kp    : Kp -> Tm
+  | Tm_Kd    : Kd -> Tm
+  | Tm_V     : V  -> Tm
+  | Tm_Comb  : Tm -> Tm -> Tm.
 derive Tm.
+Elpi derive.eqbOK.register_axiom Tm is_Tm is_nat_inhab Tm_eqb Tm_eqb_correct Tm_eqb_refl.
+HB.instance Definition _ := hasDecEq.Build Tm Tm_eqb_OK.
 
-Record R_ {A} := mkR { head : Tm; premises : list A }.
+Inductive Callable := 
+  | Callable_Kp   : Kp -> Callable
+  | Callable_V    : V -> Callable
+  | Callable_Comb : Callable -> Tm -> Callable.
+derive Callable.
+Elpi derive.eqbOK.register_axiom Callable is_Callable is_nat_inhab Callable_eqb Callable_eqb_correct Callable_eqb_refl.
+HB.instance Definition _ := hasDecEq.Build Callable Callable_eqb_OK.
+
+(* Used for rules head *)
+Inductive RCallable := 
+  | RCallable_Kp   : Kp -> RCallable
+  | RCallable_Comb : RCallable -> Tm -> RCallable.
+derive RCallable.
+Elpi derive.eqbOK.register_axiom RCallable is_RCallable is_nat_inhab RCallable_eqb RCallable_eqb_correct RCallable_eqb_refl.
+HB.instance Definition _ := hasDecEq.Build RCallable RCallable_eqb_OK.
+
+Record R_ {A} := mkR { head : RCallable; premises : list A }.
 Arguments mkR {_} _ _.
 derive R_.
 Inductive A :=
-  | Cut
-  | Call : Tm -> A.
+  | ACut
+  | ACall : Callable -> A.
 derive A.
+HB.instance Definition _ := hasDecEq.Build A A_eqb_OK.
+
 
   (* | PiImpl : V -> R_ A -> A -> A. *)
 Notation R := (@R_ A).
-
-HB.instance Definition _ := hasDecEq.Build Tm Tm_eqb_OK.
-HB.instance Definition _ := hasDecEq.Build A A_eqb_OK.
-HB.instance Definition _ := hasDecEq.Build C C_eqb_OK.
-HB.instance Definition _ := hasDecEq.Build P P_eqb_OK.
-HB.instance Definition _ := hasDecEq.Build K K_eqb_OK.
-HB.instance Definition _ := hasDecEq.Build V V_eqb_OK.
 HB.instance Definition _ := hasDecEq.Build R (R__eqb_OK _ _ A_eqb_OK).
 
 Record Sigma := { sigma : V -> option Tm }.
 Definition empty : Sigma := {| sigma := fun _ => None |}.
 
 Definition index := list R.
-Definition mode_ctx := Tm -> list mode.
-Definition sigT := P -> S.
+Definition mode_ctx := RCallable -> list mode.
+Definition sigT := Kp -> S.
 (* 
-  The predicate knows about the signature of all predicates, therefore,
+  The program knows about the signature of all predicates, therefore,
   for each predicate we return a S (not an option S)
 *)
 Record program := { (*depth : nat;*) rules : index; modes : mode_ctx; sig : sigT }.
