theories/run_test.v
@@ -3,12 +3,12 @@ From det Require Import lang run.
 
 Notation "X &&& Y" := (And X _ Y) (at level 3).
 Notation "X ||[ Y s ]" := (Or X s Y) (at level 3).
-Notation "` X" := ((Call X)) (at level 3).
+Notation "` X" := ((ACall X)) (at level 3).
 
 Definition empty_sig : sigT := fun _ => b(d Func).
 
 Definition build_progr l := {|
-    modes := (fix rec (t : Tm) := match t with Comb h _ => o :: rec h | Code _ | Data _ => [::] end);
+    modes := (fix rec t := match t with RCallable_Comb h _ => o :: rec h | RCallable_Kp _ => [::] end);
     sig := empty_sig;
     rules := l;
 |}.
@@ -16,43 +16,52 @@ Definition build_progr l := {|
 (* Section RunAxiom:= Run(UAxioms). *)
 Definition unifyF    (t1 t2 : Tm) (s : Sigma) :=
   match t1, t2 with
-  | Code (v X), _ => match s.(sigma) X with None => Some {| sigma := (fun x => if x == X then Some t2 else s.(sigma) x) |} | Some t => if t == t2 then Some s else None end
-  | _, Code (v X) => match s.(sigma) X with None => Some {| sigma := (fun x => if x == X then Some t1 else s.(sigma) x) |} | Some t => if t == t1 then Some s else None end
+  | Tm_V X, _ => match s.(sigma) X with None => Some {| sigma := (fun x => if x == X then Some t2 else s.(sigma) x) |} | Some t => if t == t2 then Some s else None end
+  | _, Tm_V X => match s.(sigma) X with None => Some {| sigma := (fun x => if x == X then Some t1 else s.(sigma) x) |} | Some t => if t == t1 then Some s else None end
   | _, _ => if t1 == t2 then Some s else None
   end.
 
 Definition matchingF (t1 t2 : Tm) (s : Sigma) := if t1 == t2 then Some s else None.
+
+Definition derefF (s:Sigma) (t1:Tm) : Tm := t1.
+
 Definition unif : Unif := {|
   unify := unifyF;
-  matching := matchingF
+  matching := matchingF;
+  deref := derefF;
 |}.
 
+Definition r := (IKp 2).
+Definition p := (IKp 1).
+Definition q := (IKp 0).
 
-Definition v_X := Code (v 0).
-Definition pred_q x  := Comb (Code (p 1)) x.
-Definition pred_p x  := Comb (Code (p 0)) x.
-Definition pred_r x  := Comb (Code (p 2)) x.
-Definition pred_fail := Code (p 100).
+Definition v_X := Tm_V (IV 0).
+Definition pred_q x  := Tm_Comb (Tm_Kp p) x.
+Definition pred_p x  := Tm_Comb (Tm_Kp q) x.
+Definition pred_r x  := Tm_Comb (Tm_Kp r) x.
+Definition pred_fail := Tm_Kp (IKp 100).
 
-Definition s1 := {| sigma := (fun x => if x == 0 then Some (Data 1) else None) |}.
-Definition s2 := {| sigma := (fun x => if x == 0 then Some (Data 2) else None) |}.
+Definition s1 := {| sigma := (fun x => if x == IV 0 then Some (Tm_Kd (IKd 1)) else None) |}.
+Definition s2 := {| sigma := (fun x => if x == IV 0 then Some (Tm_Kd (IKd 2)) else None) |}.
 
 Section Test1.
 
   Definition p_test : program := build_progr [:: 
-      mkR (pred_p (Data 1)) [::] ;
-      mkR (pred_p (Data 2)) [::] ;
-      mkR (pred_r (Data 2)) [::] ;
-      mkR (pred_q (Data 1)) [:: Call (pred_p v_X) ; Call (pred_r v_X) ] 
+      mkR (RCallable_Comb (RCallable_Kp p) (Tm_Kd (IKd 1))) [::] ;
+      mkR (RCallable_Comb (RCallable_Kp p) (Tm_Kd (IKd 2))) [::] ;
+      mkR (RCallable_Comb (RCallable_Kp r) (Tm_Kd (IKd 2))) [::] ;
+      mkR (RCallable_Comb (RCallable_Kp q) (Tm_Kd (IKd 1)))
+        [:: ACall (Callable_Comb (Callable_Kp p) v_X) ; ACall (Callable_Comb (Callable_Kp r) v_X) ] 
     ].
 
 
-  Goal exists r, runb unif empty (CallS p_test (pred_q (Data 1))) s2 r false.
+  Goal exists r, runb unif empty (CallS p_test (Callable_Comb (Callable_Kp q) (Tm_Kd (IKd 1)))) s2 r false.
   Proof.
     eexists.
     apply: run_backtrack => //.
     - apply: expanded_step => //=.
       rewrite /big_or/F/select/=.
+
       (* apply: expanded_step => //=. *)
       apply: expanded_fail => //=.
     - move=>/=. reflexivity.
@@ -79,7 +88,6 @@ Section Test1.
             apply: expanded_step => //=.
             apply: expanded_step => //=.
             apply: expanded_done => //=.
-            move=>/=.
             reflexivity.
             reflexivity.
   Qed.
@@ -87,16 +95,14 @@ End Test1.
 
 Section Test5.
 
-  Definition pred_f x  := Comb (Code (p 1)) x.
-  Definition pred_g x  := Comb (Code (p 0)) x.
-
   Definition p_test1 : program := build_progr [:: 
-      mkR (pred_f (Data 0)) [:: Call (pred_g v_X); Cut] ;
-      mkR (pred_g (Data 1)) [::];
-      mkR (pred_g (Data 2)) [::]
+      mkR (RCallable_Comb (RCallable_Kp p) (Tm_Kd (IKd 0))) 
+        [::ACall (Callable_Comb (Callable_Kp q) v_X); ACut] ;
+      mkR (RCallable_Comb (RCallable_Kp q) (Tm_Kd (IKd 1))) [::] ;
+      mkR (RCallable_Comb (RCallable_Kp q) (Tm_Kd (IKd 2))) [::] 
     ].
 
-  Goal exists r, runb unif empty (CallS p_test1 ((pred_f (Data 0)))) s1 r false /\ next_alt None r = None.
+  Goal exists r, runb unif empty (CallS p_test1 (Callable_Comb (Callable_Kp p) (Tm_Kd (IKd 0)))) s1 r false /\ next_alt None r = None.
   Proof.
     repeat eexists.
     apply: run_backtrack.
@@ -130,18 +136,18 @@ End Test5.
 
 Section Test6.
 
-  Definition pred_true := (Code (p 0)).
+  Definition pred_true := ((IKp 200)).
 
   Definition p_test2 : program := build_progr [:: 
-      mkR pred_true [::];
-      mkR (pred_f (Data 0)) [:: Call (pred_g v_X); Call pred_true; Cut] ;
-      mkR (pred_g (Data 1)) [::];
-      mkR (pred_g (Data 2)) [::]
+      mkR ((RCallable_Kp pred_true)) [::];
+      mkR (RCallable_Comb (RCallable_Kp p) (Tm_Kd (IKd 0))) 
+        [::ACall (Callable_Comb (Callable_Kp q) v_X);ACall ((Callable_Kp pred_true)); ACut] ;
+      mkR (RCallable_Comb (RCallable_Kp q) (Tm_Kd (IKd 1))) [::] ;
+      mkR (RCallable_Comb (RCallable_Kp q) (Tm_Kd (IKd 2))) [::] 
   ].
 
-  (* Notation "[ x -> _]" := {| sigma := (fun x : V => _) |} (x binder). *)
-
-  Goal exists r, runb unif empty (CallS p_test2 ((pred_f (Data 0)))) s1 r false /\ next_alt None r = None.
+  Goal exists r, 
+    runb unif empty ((CallS p_test2 (Callable_Comb (Callable_Kp p) (Tm_Kd (IKd 0)))) ) s1 r false /\ next_alt None r = None.
   Proof.
     repeat eexists.
     apply: run_backtrack.
